x86model/Model/Decode.v
@@ -1987,11 +1987,11 @@ Definition SFENCE_p := "0000" $$ "1111" $$ "1010" $$ "1110" $$ "1111" $$
      (fun p => match p with (l, (s, op)) =>
                  mkPrefix l s (opt2b op false) false %% prefix_t end).
 
-   (* this set of instructions can take prefixes in prefix_grammar_rep;
-     that is, in lock_or_rep, only rep can be used;
-     we put RET in this category because it turns out many binaries use
-     the "rep ret" sequence to avoid branch prediction panelty in AMD processors;
-     intel processor seems to just ignore the rep prefix *)
+  (** this set of instructions can take prefixes in prefix_grammar_rep;
+     that is, in lock_or_rep, only rep can be used; we put RET in this
+     category because it turns out many binaries use "rep ret" to avoid the
+     branch prediction panelty in AMD processors; intel processor seems to
+     just ignore the rep prefix in "rep ret". *)
   Definition instr_grammars_rep :=
     INS_p :: OUTS_p :: MOVS_p :: LODS_p :: STOS_p :: RET_p :: nil.
 
@@ -2009,10 +2009,10 @@ Definition SFENCE_p := "0000" $$ "1111" $$ "1010" $$ "1110" $$ "1111" $$
      (fun p => match p with (l, (s, op)) =>
                  mkPrefix l s op false %% prefix_t end).
 
-  (* this set of instructions can take prefixes in 
-     prefix_grammar_lock_with_op_override;
-     that is, in lock_or_rep, only lock can be used;
-     and op_override prefix *must* be used *)
+  (** Instructions that can take prefixes in
+     prefix_grammar_lock_with_op_override: in lock_or_rep, only lock can be
+     used; segment override is optional; op_override prefix *must* be used
+     *)
   Definition instr_grammars_lock_with_op_override := 
     ADD_p true :: ADC_p true :: AND_p true :: NEG_p :: NOT_p :: OR_p true
     :: SBB_p true :: SUB_p true :: XOR_p true :: XCHG_p :: nil.
@@ -2022,10 +2022,10 @@ Definition SFENCE_p := "0000" $$ "1111" $$ "1010" $$ "1110" $$ "1111" $$
      (fun p => match p with (l, s) =>
                  mkPrefix l s false false %% prefix_t end).
 
-  (* this set of instructions can take prefixes in 
-     prefix_grammar_lock_no_op_override;
-     that is, in lock_or_rep, only lock can be used;
-     and op_override prefix *must not* be used *)
+  (** Instructions that can take prefixes in
+     prefix_grammar_lock_no_op_override; that is, in lock_or_rep, only lock
+     can be used; segment override is optional; and op_override prefix
+     *must not* be used *)
   Definition instr_grammars_lock_no_op_override := 
     ADD_p false :: ADC_p false :: AND_p false :: BTC_p :: BTR_p :: 
     BTS_p :: CMPXCHG_p :: DEC_p :: INC_p :: NEG_p :: NOT_p :: OR_p false
@@ -2122,8 +2122,9 @@ Definition SFENCE_p := "0000" $$ "1111" $$ "1010" $$ "1110" $$ "1111" $$
     unfold num_tokens. rewrite H. apply Z2Nat.inj_lt ; auto. omega.
   Qed.
 
-  Definition parse_byte (ps:instParserState (Pair_t prefix_t instruction_t))
-                         (byte:int8) : 
+  Definition ParseState_t := instParserState (Pair_t prefix_t instruction_t).
+
+  Definition parse_byte (ps: ParseState_t) (byte:int8) : 
     instParserState (Pair_t prefix_t instruction_t) * list (prefix * instr) := 
     parse_token ps (byte_less_than_num_tokens byte).
 
